common/AST.v
@@ -56,7 +56,7 @@ Definition Tptr : typ := if Archi.ptr64 then Tlong else Tint.
 Definition typesize (ty: typ) : Z :=
   match ty with
   | Tint => 4
-  | Tfloat => 8
+  | Tfloat => 4
   | Tlong => 8
   | Tsingle => 4
   | Tany32 => 4
@@ -79,7 +79,7 @@ Definition subtype (ty1 ty2: typ) : bool :=
   | Tlong, Tlong => true
   | Tfloat, Tfloat => true
   | Tsingle, Tsingle => true
-  | (Tint | Tsingle | Tany32), Tany32 => true
+  | (Tint | Tsingle | Tfloat | Tany32), Tany32 => true
   | _, Tany64 => true
   | _, _ => false
   end.
@@ -147,8 +147,8 @@ Inductive memory_chunk : Type :=
   | Mint16unsigned  (**r 16-bit unsigned integer *)
   | Mint32          (**r 32-bit integer, or pointer *)
   | Mint64          (**r 64-bit integer *)
-  | Mfloat32        (**r 32-bit single-precision float *)
-  | Mfloat64        (**r 64-bit double-precision float *)
+  | Mfloat32s       (**r 32-bit single-precision float *)
+  | Mfloat32d       (**r double type from C is 32-bit on Patmos *)
   | Many32          (**r any value that fits in 32 bits *)
   | Many64.         (**r any value *)
 
@@ -168,8 +168,8 @@ Definition type_of_chunk (c: memory_chunk) : typ :=
   | Mint16unsigned => Tint
   | Mint32 => Tint
   | Mint64 => Tlong
-  | Mfloat32 => Tsingle
-  | Mfloat64 => Tfloat
+  | Mfloat32s => Tsingle
+  | Mfloat32d => Tfloat
   | Many32 => Tany32
   | Many64 => Tany64
   end.
@@ -183,9 +183,9 @@ Proof. unfold Mptr, Tptr; destruct Archi.ptr64; auto. Qed.
 Definition chunk_of_type (ty: typ) :=
   match ty with
   | Tint => Mint32
-  | Tfloat => Mfloat64
+  | Tfloat => Mfloat32d
   | Tlong => Mint64
-  | Tsingle => Mfloat32
+  | Tsingle => Mfloat32s
   | Tany32 => Many32
   | Tany64 => Many64
   end.
@@ -200,8 +200,8 @@ Inductive init_data: Type :=
   | Init_int16: int -> init_data
   | Init_int32: int -> init_data
   | Init_int64: int64 -> init_data
-  | Init_float32: float32 -> init_data
-  | Init_float64: float -> init_data
+  | Init_float32s: float32 -> init_data
+  | Init_float32d: float32 -> init_data
   | Init_space: Z -> init_data
   | Init_addrof: ident -> ptrofs -> init_data.  (**r address of symbol + offset *)
 
@@ -211,8 +211,8 @@ Definition init_data_size (i: init_data) : Z :=
   | Init_int16 _ => 2
   | Init_int32 _ => 4
   | Init_int64 _ => 8
-  | Init_float32 _ => 4
-  | Init_float64 _ => 8
+  | Init_float32s _ => 4
+  | Init_float32d _ => 4
   | Init_addrof _ _ => if Archi.ptr64 then 8 else 4
   | Init_space n => Z.max n 0
   end.
@@ -621,7 +621,7 @@ Inductive builtin_arg (A: Type) : Type :=
   | BA (x: A)
   | BA_int (n: int)
   | BA_long (n: int64)
-  | BA_float (f: float)
+  | BA_float (f: float32)
   | BA_single (f: float32)
   | BA_loadstack (chunk: memory_chunk) (ofs: ptrofs)
   | BA_addrstack (ofs: ptrofs)
